theories/c_lang/class_instances.v
@@ -11,8 +11,8 @@ Section pure_exec.
     subst; intros ?; apply nsteps_once, pure_head_step_pure_step;
       constructor; [solve_exec_safe | solve_exec_puredet].
 
-  Local Ltac destruct_bool_decide := repeat (let H := fresh "Heq" in 
-    try destruct bool_decide eqn:H; 
+  Local Ltac destruct_bool_decide := repeat (let H := fresh "Heq" in
+    try destruct bool_decide eqn:H;
     [apply bool_decide_eq_true_1 in H| apply bool_decide_eq_false_1 in H]).
 
   Global Instance pure_unop op v v' :
@@ -35,27 +35,28 @@ Section pure_exec.
   Global Instance pure_if_false v e1 e2 : asTruth v = false ->
     PureExec True 1 p (If (Val $ v) e1 e2) e2.
   Proof. intros H. solve_pure_exec. congruence. Qed.
-  Global Instance pure_if_zero e1 e2 : 
+  Global Instance pure_if_zero e1 e2 :
     PureExec True 1 p (If (Val $ LitV $ LitInt (0%Z)) e1 e2) e2.
   Proof. apply pure_if_false. easy. Qed.
   Global Instance pure_if_false_bool e1 e2 :
     PureExec True 1 p (If (Val $ LitV $ LitBool false) e1 e2) e2.
   Proof. apply pure_if_zero. Qed.
 
-  Global Instance pure_while e1 e2 : 
+  Global Instance pure_while e1 e2 :
     PureExec True 1 p (While e1 e2) (If e1 (Let BAnon e2 (While e1 e2)) (Val $ LitV $ LitInt 0)).
   Proof. solve_pure_exec. Qed.
 
-  Global Instance pure_let x (v1:val) e2 : 
-    PureExec True 1 p (Let x v1 e2) (subst' x v1 e2).
+  Global Instance pure_let x v1 e2 :
+    PureExec True 1 p (Let x (Val v1) e2) (subst_var x (Val v1) e2).
   Proof. solve_pure_exec. Qed.
 
-  Global Instance pure_funcall s va args res e : 
-    PureExec ((p : gmap.gmap string function) !! s = Some (Fun args e) ∧ zip_args args va = Some res) 1 p (FunCall (Val $ LitV $ LitFunPtr s) (map Val va)) (subst_all res e).
+  Global Instance pure_funcall s va args res e :
+    PureExec
+      ((p : gmap.gmap string function) !! s = Some (Fun args e) ∧ zip_args args va = Some res)
+      1 p (FunCall (Val $ LitV $ LitFunPtr s) (map Val va)) (subst_all res ∅ e).
   Proof. solve_pure_exec; destruct H as [H1 H2].
     1: econstructor; first done.
     + unfold apply_function. rewrite H2. reflexivity.
-    + repeat split; try congruence. destruct (zip_args args0 va) eqn:Heq; last congruence.
-      congruence.
+    + repeat split. destruct (zip_args args0 va) eqn:Heq; congruence.
   Qed.
 End pure_exec.
