theories/c_lang/lang_instantiation.v
@@ -6,6 +6,7 @@ From iris.prelude Require Import options.
 From melocoton Require Import stdpp_extra.
 From melocoton.language Require Import language.
 From melocoton.c_interface Require Import defs.
+From melocoton.c_lang Require Export lang.
 
 Local Notation state := (gmap loc heap_cell).
 
